src/protocol/DNS.Protocol.Parser.EverParseAdapter.fst
@@ -152,10 +152,12 @@ let generated_dns_uncompressed_question_txt_answer_packet_validator
     rdata_length
 
 let generated_dns_uncompressed_question_compressed_answer_name_packet_validator
-    qname_length rdata_length =
+    qname_length rdata_length rr_name_ptr_hi_value rr_name_ptr_lo_value =
   DNSProtocol.validate__dns_uncompressed_question_compressed_answer_name_packet
     qname_length
     rdata_length
+    rr_name_ptr_hi_value
+    rr_name_ptr_lo_value
 
 let generated_dns_opt_additional_packet_validator option_payload_length =
   DNSProtocol.validate__dns_opt_additional_packet option_payload_length
